Interface changes for Poly1305_32

code/poly1305_32/Hacl.Poly1305_32.fsti
@@ -1,9 +1,7 @@
 module Hacl.Poly1305_32
 
+open FStar.HyperStack
 open FStar.HyperStack.All
-
-module ST = FStar.HyperStack.ST
-
 open FStar.Mul
 open FStar.Endianness
 open FStar.Buffer
@@ -11,13 +9,82 @@ open FStar.UInt64
 
 open Hacl.Spec.Endianness
 
+module I = Hacl.Impl.Poly1305_32
+module S = Hacl.Spec.Poly1305_32
+module ST = FStar.HyperStack.ST
+module A = Hacl.Spec.Bignum.AddAndMultiply
+
+
 #reset-options "--max_fuel 0 --z3rlimit 100"
 
 (* Type Aliases *)
 let uint8_p = Buffer.buffer Hacl.UInt8.t
 let uint64_t = FStar.UInt64.t
-let op_String_Access h (b:uint8_p{live h b}) = reveal_sbytes (as_seq h b)
+private let op_String_Access h (b:uint8_p{live h b}) = reveal_sbytes (as_seq h b)
 
+(* Type Aliases *)
+private type key = k:uint8_p{length k = 32}
+
+private type state = I.poly1305_state
+private type live_state (h:mem) (st:state) = I.live_st h st
+private type stable (h:mem) (st:state) = live_state h st /\ S.red_y (as_seq h I.(st.h)) /\ S.red_26 (as_seq h I.(st.r))
+
+private let get_key (st:state) = I.(st.r)
+private let get_accumulator (st:state) = I.(st.h)
+
+#reset-options "--initial_fuel 0 --max_fuel 0 --z3rlimit 100"
+
+val alloc:
+  unit -> StackInline state
+    (requires (fun h -> True))
+    (ensures (fun h0 st h1 -> modifies_0 h0 h1 /\ I.live_st h1 st /\ frameOf I.(st.h) == h0.tip
+      /\ frameOf I.(st.r) = h0.tip /\ (I.(st.r) `unused_in` h0) /\ (I.(st.h) `unused_in` h0)))
+
+val mk_state:
+  r:buffer Hacl.UInt32.t{length r = 5} -> acc:buffer Hacl.UInt32.t{length acc = 5 /\ disjoint r acc} ->
+  Stack state
+    (requires (fun h -> live h r /\ live h acc))
+    (ensures (fun h0 st h1 -> h0 == h1 /\ I.(st.r) == r /\ I.(st.h) == acc /\ I.live_st h1 st))
+
+val init:
+  st:state ->
+  k:uint8_p{length k >= 16} ->
+  Stack unit
+    (requires (fun h -> live h k /\ live_state h st))
+    (ensures (fun h0 _ h1 -> modifies_2 (get_key st) (get_accumulator st) h0 h1 /\ stable h1 st))
+
+val update_block:
+  st:state ->
+  m:uint8_p{length m = 16} ->
+  Stack unit
+    (requires (fun h -> stable h st /\ live h m))
+    (ensures  (fun h0 updated_log h1 -> modifies_1 (get_accumulator st) h0 h1 /\ stable h1 st))
+
+val update:
+  st:state ->
+  m:uint8_p ->
+  len:FStar.UInt32.t{length m >= 16 * UInt32.v len} ->
+  Stack unit
+    (requires (fun h -> stable h st /\ live h m))
+    (ensures  (fun h0 updated_log h1 -> modifies_1 (get_accumulator st) h0 h1 /\ stable h1 st))
+
+type before_finish h st = A.(live_state h st /\ bounds (as_seq h (get_accumulator st)) p26 p26 p26 p26 p26)
+
+val update_last:
+  st:state ->
+  m:uint8_p ->
+  len:UInt32.t{UInt32.v len < 16 /\ UInt32.v len <= length m} ->
+  Stack unit
+    (requires (fun h -> stable h st /\ live h m))
+    (ensures  (fun h0 _ h1 -> modifies_1 (get_accumulator st) h0 h1 /\ before_finish h1 st))
+
+val finish:
+  st:state ->
+  mac:uint8_p{length mac = 16} ->
+  k:uint8_p{length k = 16} ->
+  Stack unit
+    (requires (fun h -> before_finish h st /\ live h mac /\ live h k))
+    (ensures (fun h0 _ h1 -> modifies_1 mac h0 h1))
 
 val crypto_onetimeauth:
   mac:uint8_p{length mac = 16} ->
